Added syntax for upshift modality

theories/Core/Syntactic/Syntax.v
@@ -1,62 +1,71 @@
 From Coq Require Import List String.
-From Coq Require Import Program.Equality.
+From Coq Require Import Program.Equality Logic.PropExtensionality.
 From McPTS Require Import PtsSignature.
 From McPTS.Core Require Import Base.
 
 
-(** * Abstract Syntax Tree *)
-Inductive exp (P : PtsSig) : Set :=
+(** * Abstract Syntax Tree *)  
+Inductive exp (P : AdjSig) : Modes P -> Set :=
 (** Sorts *)
-| a_st : P -> exp P
+| a_st : forall (m : Modes P), St m -> exp P m
 (** Functions *)
-| a_pi : forall (s1 s2 s3 : P), Ru_pi P s1 s2 s3 -> exp P -> exp P -> exp P
-| a_fn : forall (s1 s2 s3 : P), Ru_pi P s1 s2 s3 -> exp P -> exp P -> exp P -> exp P
-| a_app : exp P -> exp P -> exp P
+| a_pi : forall (m : Modes P) (s1 s2 s3 : m), Ru_pi m s1 s2 s3 -> exp P m -> exp P m -> exp P m
+| a_fn : forall (m : Modes P) (s1 s2 s3 : m), Ru_pi m s1 s2 s3 -> exp P m -> exp P m -> exp P m -> exp P m
+| a_app : forall m, exp P m -> exp P m -> exp P m
 (** Variable *)
-| a_var : nat -> exp P
+| a_var : forall m, nat -> exp P m
 (** Substitution Application *)
-| a_sub : exp P -> sub P -> exp P
+| a_sub : forall m, exp P m -> sub P -> exp P m
 (** Naturals **)
-| a_nat : exp P
-| a_zero : exp P
-| a_succ : exp P -> exp P
-| a_natrec : exp P -> exp P -> exp P -> exp P -> exp P
-with sub (P : PtsSig) : Set :=
+| a_nat : forall m, exp P m
+| a_zero : forall m, exp P m
+| a_succ : forall m, exp P m -> exp P m
+| a_natrec : forall m, exp P m -> exp P m -> exp P m -> exp P m -> exp P m
+(** Upshift *)
+| a_upshift : forall l h (leq : {{ l ⪯ h ∈ P }}) sl sh, Ru_upshift P l h leq sl sh -> exp P l -> exp P h
+| a_susp : forall l h (leq : {{ l ⪯ h ∈ P }}) sl sh, Ru_upshift P l h leq sl sh -> exp P l -> exp P h
+| a_force : forall l h (leq : {{ l ⪯ h ∈ P }}) sl sh, Ru_upshift P l h leq sl sh -> exp P h -> exp P l 
+
+with sub (P : AdjSig) : Set :=
 | a_id : sub P
 | a_weaken : sub P
 | a_compose : sub P -> sub P -> sub P
-| a_extend : sub P -> exp P -> sub P.
+| a_extend : forall m, sub P -> exp P m -> sub P.
 
-(* Make the signature implicit to all constructors *)
-Arguments a_st {_}.
-Arguments a_pi {_ _ _ _}.
-Arguments a_fn {_ _ _ _}.
-Arguments a_app {_}.
-Arguments a_var {_}.
-Arguments a_sub {_}.
-Arguments a_nat {_}.
-Arguments a_zero {_}.
-Arguments a_succ {_}.
-Arguments a_natrec {_}.
+
+(* Make the adjoint signature implicit to all constructors *)
+Arguments a_st {_ _}.
+Arguments a_pi {_ _ _ _ _}.
+Arguments a_fn {_ _ _ _ _}.
+Arguments a_app {_ _}.
+Arguments a_var {_ _}.
+Arguments a_sub {_ _}.
+Arguments a_nat {_ _}.
+Arguments a_zero {_ _}.
+Arguments a_succ {_ _}.
+Arguments a_natrec {_ _}.
+Arguments a_upshift {_ _ _ _ _ _}.
+Arguments a_susp {_ _ _ _ _ _}.
+Arguments a_force {_ _ _ _ _ _}.
 Arguments a_id {_}.
 Arguments a_weaken {_}.
 Arguments a_compose {_}.
-Arguments a_extend {_}.
+Arguments a_extend {_ _}.
 
 
-Notation typ := (fun P => exp P).
-Notation ctx := (fun (P : PtsSig) => list (typ P)%type).
+Notation typ := (fun P m => exp P m).
+Notation ctx := (fun P m => list (typ P m)).
 
-Fixpoint nat_to_exp {P : PtsSig} (n : nat) : exp P :=
+Fixpoint nat_to_exp {P : AdjSig} {m : Modes P} (n : nat) : exp P m :=
   match n with
   | 0 => a_zero
   | S m => a_succ (nat_to_exp m)
   end.
 
-Definition num_to_exp {P : PtsSig} (n : Number.uint) : exp P :=
+Definition num_to_exp {P : AdjSig} {m : Modes P} (n : Number.uint) : exp P m :=
   nat_to_exp (Nat.of_num_uint n).
 
-Fixpoint exp_to_nat {P : PtsSig} (e : exp P) : option nat :=
+Fixpoint exp_to_nat {P : AdjSig} {m : Modes P} (e : exp P m) : option nat :=
   match e with
   | a_zero => Some 0
   | a_succ e' =>
@@ -67,7 +76,7 @@ Fixpoint exp_to_nat {P : PtsSig} (e : exp P) : option nat :=
   | _ => None
   end.
 
-Definition exp_to_num {P : PtsSig} (e : exp P) :=
+Definition exp_to_num {P : AdjSig} {m : Modes P} (e : exp P m) :=
   match exp_to_nat e with
   | Some n => Some (Nat.to_num_uint n)
   | None => None
@@ -81,33 +90,39 @@ Combined Scheme syntax_mut_ind from
   sub_mut_ind.
 
 (** ** Syntactic Normal/Neutral Form *)
-Inductive nf (P : PtsSig) : Set :=
-| nf_st : P -> nf P
-| nf_pi : forall (s1 s2 s3 : P), Ru_pi P s1 s2 s3 -> nf P -> nf P -> nf P
-| nf_fn : forall (s1 s2 s3 : P), Ru_pi P s1 s2 s3 -> nf P -> nf P -> nf P -> nf P
-| nf_nat : nf P
-| nf_zero : nf P
-| nf_succ : nf P -> nf P
-| nf_neut : ne P -> nf P
-with ne (P : PtsSig) : Set :=
-| ne_app : ne P -> nf P -> ne P
-| ne_var : nat -> ne P
-| ne_natrec : nf P -> nf P -> nf P -> ne P -> ne P
+Inductive nf (P : AdjSig) : Modes P -> Set :=
+| nf_st : forall (m : Modes P), St m -> nf P m
+| nf_pi : forall (m : Modes P) (s1 s2 s3 : m), Ru_pi m s1 s2 s3 -> nf P m -> nf P m -> nf P m
+| nf_fn : forall (m : Modes P) (s1 s2 s3 : m), Ru_pi m s1 s2 s3 -> nf P m -> nf P m -> nf P m -> nf P m
+| nf_nat : forall m, nf P m
+| nf_zero : forall m, nf P m
+| nf_succ : forall m, nf P m -> nf P m
+| nf_neut : forall m, ne P m -> nf P m
+| nf_upshift : forall l h (leq : {{ l ⪯ h ∈ P }}) sl sh, Ru_upshift P l h leq sl sh -> nf P l -> nf P h
+| nf_susp : forall l h (leq : {{ l ⪯ h ∈ P }}) sl sh, Ru_upshift P l h leq sl sh -> nf P l -> nf P h
+with ne (P : AdjSig) : Modes P -> Set :=
+| ne_app : forall m, ne P m -> nf P m -> ne P m
+| ne_var : forall m, nat -> ne P m
+| ne_natrec : forall m, nf P m -> nf P m -> nf P m -> ne P m -> ne P m
+| ne_force : forall l h (leq : {{ l ⪯ h ∈ P }}) sl sh, Ru_upshift P l h leq sl sh -> ne P h -> ne P l
 .
 
-Arguments nf_st {_}.
-Arguments nf_pi {_ _ _ _}.
-Arguments nf_fn {_ _ _ _}.
-Arguments nf_nat {_}.
-Arguments nf_zero {_}.
-Arguments nf_succ {_}.
-Arguments nf_neut {_}.
+Arguments nf_st {_ _}.
+Arguments nf_pi {_ _ _ _ _}.
+Arguments nf_fn {_ _ _ _ _}.
+Arguments nf_nat {_ _}.
+Arguments nf_zero {_ _}.
+Arguments nf_succ {_ _}.
+Arguments nf_neut {_ _}.
+Arguments nf_upshift {_ _ _ _ _ _}.
+Arguments nf_susp {_ _ _ _ _ _}.
 
-Arguments ne_app {_}.
-Arguments ne_var {_}.
-Arguments ne_natrec {_}.
+Arguments ne_app {_ _}.
+Arguments ne_var {_ _}.
+Arguments ne_natrec {_ _}.
+Arguments ne_force {_ _ _ _ _ _}.
 
-Fixpoint nf_to_exp {P : PtsSig} (M : nf P) : exp P :=
+Fixpoint nf_to_exp {P : AdjSig} {m : Modes P} (M : nf P m) : exp P m :=
   match M with
   | nf_st s => a_st s
   | nf_pi r A B => a_pi r (nf_to_exp A) (nf_to_exp B)
@@ -116,78 +131,164 @@ Fixpoint nf_to_exp {P : PtsSig} (M : nf P) : exp P :=
   | nf_zero => a_zero
   | nf_succ M => a_succ (nf_to_exp M)
   | nf_neut M => ne_to_exp M
+  | nf_upshift r A => a_upshift r (nf_to_exp A)
+  | nf_susp r M => a_susp r (nf_to_exp M)
   end
-with ne_to_exp {P : PtsSig} (M : ne P) : exp P :=
+with ne_to_exp {P : AdjSig} {m : Modes P} (M : ne P m) : exp P m :=
   match M with
   | ne_app M N => a_app (ne_to_exp M) (nf_to_exp N)
   | ne_var x => a_var x
   | ne_natrec A MZ MS M => a_natrec (nf_to_exp A) (nf_to_exp MZ) (nf_to_exp MS) (ne_to_exp M)
+  | ne_force r M => a_force r (ne_to_exp M)
   end
 .
 
 Coercion nf_to_exp : nf >-> exp.
 Coercion ne_to_exp : ne >-> exp.
-  
-Fact nf_eq_dec {P : PtsSig} (dec_P : DecidableSig P) : forall (M M' : nf P),
-    ({M = M'} + {M <> M'})%type
-with ne_eq_dec {P : PtsSig} (dec_P : DecidableSig P): forall (M M' : ne P),
-    ({M = M'} + {M <> M'})%type.
-Proof.
-  - intros.
-    destruct M; destruct M';
-      try solve [right; intros H; inversion H];
-      try solve [left; reflexivity].
-    + destruct (dec_st_eq dec_P s s0).
-      * subst.
-        left.
-        reflexivity.
-      * right.
-        injection.
-        eassumption.
-    + destruct (dec_st_eq dec_P s1 s0); [| right; injection; intros; auto].
-      destruct (dec_st_eq dec_P s2 s4); [| right; injection; intros; auto].
-      destruct (dec_st_eq dec_P s3 s5); [| right; injection; intros; auto].
-      subst.
-      pose proof (dec_ru_pi_eq dec_P _ _ _ r r0).
-      destruct H; [| right; injection; intros; simpl_existTs; auto].
-      subst.
-      destruct (nf_eq_dec P dec_P M1 M'1); [| right; injection; auto].
-      destruct (nf_eq_dec P dec_P M2 M'2); [| right; injection; auto].
-      subst.
-      left.
-      reflexivity.
-    + destruct (dec_st_eq dec_P s1 s0); [| right; injection; intros; auto].
-      destruct (dec_st_eq dec_P s2 s4); [| right; injection; intros; auto].
-      destruct (dec_st_eq dec_P s3 s5); [| right; injection; intros; auto].
-      subst.
-      pose proof (dec_ru_pi_eq dec_P _ _ _ r r0).
-      destruct H; [| right; injection; intros; simpl_existTs; auto].
-      subst.
-      destruct (nf_eq_dec P dec_P M1 M'1); [| right; injection; auto].
-      destruct (nf_eq_dec P dec_P M2 M'2); [| right; injection; auto].
-      destruct (nf_eq_dec P dec_P M3 M'3); [| right; injection; auto].
-      subst.
-      left.
-      reflexivity.
-    + destruct (nf_eq_dec P dec_P M M').
-      * subst.
-        left.
-        reflexivity.
-      * right.
-        injection.
-        eassumption.
-    + destruct (ne_eq_dec P dec_P n n0).
-      * subst.
-        left.
-        reflexivity.
-      * right.
-        injection.
-        eassumption.
-  - intros; decide equality; try apply PeanoNat.Nat.eq_dec.
-Defined.
 
-Definition q {P : PtsSig} (σ : sub P) := a_extend (a_compose σ a_weaken) (a_var 0).
-Arguments q {_} σ/.
+Section DecideNfEq.
+  Lemma eq_upshift_implies_strong_ru_upshift_eq {P : AdjSig} (dec_P : DecidableAdjSig P) :
+    forall l l' h (leq : Mode_preorder P l h) (leq' : Mode_preorder P l' h) sl sl' sh sh' (r : Ru_upshift P l h leq sl sh) (r' : Ru_upshift P l' h leq' sl' sh') A A',
+      (nf_upshift r A = nf_upshift r' A') ->
+      strong_ru_upshift_eq l l' h h leq leq' sl sl' sh sh' r r'.
+  Proof.
+    intros.
+    inversion H; subst.
+    assert (leq = leq') as -> by (apply proof_irrelevance).
+    simpl_existTs; subst.
+    simpl_existTs; subst.
+    repeat split; reflexivity.
+  Qed.
+
+  Lemma eq_susp_implies_strong_ru_upshift_eq {P : AdjSig} (dec_P : DecidableAdjSig P) :
+    forall l l' h (leq : Mode_preorder P l h) (leq' : Mode_preorder P l' h) sl sl' sh sh' (r : Ru_upshift P l h leq sl sh) (r' : Ru_upshift P l' h leq' sl' sh') M M',
+      (nf_susp r M = nf_susp r' M') ->
+      strong_ru_upshift_eq l l' h h leq leq' sl sl' sh sh' r r'.
+  Proof.
+    intros.
+    inversion H; subst.
+    assert (leq = leq') as -> by (apply proof_irrelevance).
+    simpl_existTs; subst.
+    simpl_existTs; subst.
+    repeat split; reflexivity.
+  Qed.
+
+  Lemma eq_force_implies_strong_ru_upshift_eq {P : AdjSig} (dec_P : DecidableAdjSig P) :
+    forall l h h' (leq : Mode_preorder P l h) (leq' : Mode_preorder P l h') sl sl' sh sh' (r : Ru_upshift P l h leq sl sh) (r' : Ru_upshift P l h' leq' sl' sh') M M',
+      (ne_force r M = ne_force r' M') ->
+      strong_ru_upshift_eq l l h h' leq leq' sl sl' sh sh' r r'.
+  Proof.
+    intros.
+    inversion H; subst.
+    assert (leq = leq') as -> by (apply proof_irrelevance).
+    simpl_existTs; subst.
+    simpl_existTs; subst.
+    repeat split; reflexivity.
+  Qed.
+  
+  Fact nf_eq_dec {P : AdjSig} (dec_P : DecidableAdjSig P) : forall (m : Modes P) (M M' : nf P m),
+      ({M = M'} + {M <> M'})%type
+      with ne_eq_dec {P : AdjSig} (dec_P : DecidableAdjSig P): forall (m : Modes P) (M M' : ne P m),
+          ({M = M'} + {M <> M'})%type.
+  Proof.
+    - intros.
+      pose proof (dec_sigs dec_P m) as dec_m.
+      destruct M; destruct M';
+        try solve [right; intros H; inversion H];
+        try solve [left; reflexivity].
+      + destruct (dec_st_eq dec_m s s0).
+        * subst.
+          left.
+          reflexivity.
+        * right.
+          injection.
+          intros.
+          simpl_existTs.
+          intuition.
+      + destruct (dec_st_eq dec_m s1 s0); [| right; injection; intros; simpl_existTs; auto].
+        destruct (dec_st_eq dec_m s2 s4); [| right; injection; intros; simpl_existTs; auto].
+        destruct (dec_st_eq dec_m s3 s5); [| right; injection; intros; simpl_existTs; auto].
+        subst.
+        destruct (dec_ru_pi_eq dec_m _ _ _ r r0); [| right; injection; intros; simpl_existTs; auto].
+        subst.
+        destruct (nf_eq_dec P dec_P m M1 M'1); [| right; injection; intros; simpl_existTs; auto].
+        destruct (nf_eq_dec P dec_P m M2 M'2); [| right; injection; intros; simpl_existTs; auto].
+        subst.
+        left.
+        reflexivity.
+      + destruct (dec_st_eq dec_m s1 s0); [| right; injection; intros; simpl_existTs; auto].
+        destruct (dec_st_eq dec_m s2 s4); [| right; injection; intros; simpl_existTs; auto].
+        destruct (dec_st_eq dec_m s3 s5); [| right; injection; intros; simpl_existTs; auto].
+        subst.
+        destruct (dec_ru_pi_eq dec_m _ _ _ r r0); [| right; injection; intros; simpl_existTs; auto].
+        subst.
+        destruct (nf_eq_dec P dec_P m M1 M'1); [| right; injection; intros; simpl_existTs; auto].
+        destruct (nf_eq_dec P dec_P m M2 M'2); [| right; injection; intros; simpl_existTs; auto].
+        destruct (nf_eq_dec P dec_P m M3 M'3); [| right; injection; intros; simpl_existTs; auto].
+        subst.
+        left.
+        reflexivity.
+      + destruct (nf_eq_dec P dec_P m M M').
+        * subst.
+          left.
+          reflexivity.
+        * right.
+          injection.
+          intros.
+          simpl_existTs.
+          auto.
+      + destruct (ne_eq_dec P dec_P m n n0).
+        * subst.
+          left.
+          reflexivity.
+        * right.
+          injection.
+          intros.
+          simpl_existTs.
+          auto.
+      + destruct (strong_dec_ru_upshift dec_P l l0 h h leq leq0 sl sl0 sh sh0 r r0).
+        * destruct s as [Hl [Hh [Hleq [Hsl [Hsh Hr]]]]]; subst.
+          destruct (nf_eq_dec P dec_P l0 M M'); [| right; injection; intros; simpl_existTs; auto].
+          left; subst; reflexivity.
+        * right; injection.
+          assert (strong_ru_upshift_eq l l0 h h leq leq0 sl sl0 sh sh0 r r0) by (eapply eq_upshift_implies_strong_ru_upshift_eq; eauto).
+          auto.
+      + destruct (strong_dec_ru_upshift dec_P l l0 h h leq leq0 sl sl0 sh sh0 r r0).
+        * destruct s as [Hl [Hh [Hleq [Hsl [Hsh Hr]]]]]; subst.
+          destruct (nf_eq_dec P dec_P l0 M M'); [| right; injection; intros; simpl_existTs; auto].
+          left; subst; reflexivity.
+        * right; injection.
+          assert (strong_ru_upshift_eq l l0 h h leq leq0 sl sl0 sh sh0 r r0) by (eapply eq_susp_implies_strong_ru_upshift_eq; eauto).
+          auto.
+          
+    - intros.
+      pose proof (dec_sigs dec_P m) as dec_m.
+      destruct M; destruct M';
+        try solve [right; intros H; inversion H];
+        try solve [left; reflexivity].
+      + destruct (ne_eq_dec P dec_P m M M'); [| right; injection; intros; simpl_existTs; auto].
+        destruct (nf_eq_dec P dec_P m n n0); [| right; injection; intros; simpl_existTs; auto].
+        left; subst; reflexivity.
+      + destruct (PeanoNat.Nat.eq_dec n n0); [| right; injection; intros; auto].
+        left; subst; reflexivity.
+      + destruct (ne_eq_dec P dec_P m M M'); [| right; injection; intros; simpl_existTs; auto].
+        destruct (nf_eq_dec P dec_P m n n2); [| right; injection; intros; simpl_existTs; auto].
+        destruct (nf_eq_dec P dec_P m n0 n3); [| right; injection; intros; simpl_existTs; auto].
+        destruct (nf_eq_dec P dec_P m n1 n4); [| right; injection; intros; simpl_existTs; auto].
+        left; subst; reflexivity.
+      + destruct (strong_dec_ru_upshift dec_P l l h h0 leq leq0 sl sl0 sh sh0 r r0).
+        * destruct s as [Hl [Hh [Hleq [Hsl [Hsh Hr]]]]]; subst.
+          destruct (ne_eq_dec P dec_P h0 M M'); [| right; injection; intros; simpl_existTs; auto].
+          left; subst; reflexivity.
+        * right; injection.
+          assert (strong_ru_upshift_eq l l h h0 leq leq0 sl sl0 sh sh0 r r0) by (eapply eq_force_implies_strong_ru_upshift_eq; eauto).
+          auto.
+  Defined.
+End DecideNfEq.
+
+
+Definition q {P : AdjSig} {m : Modes P} (σ : sub P) := a_extend (a_compose σ a_weaken) (@a_var P m 0).
+Arguments q {_} {_} σ/.
 
 
 #[global] Declare Custom Entry exp.
@@ -218,8 +319,11 @@ Module Syntax_Notations.
   Notation "'Π' r A B" := (a_pi r A B) (in custom exp at level 1, r constr at level 0, A custom exp at level 0, B custom exp at level 60) : mcpts_scope.
   Notation "'λ' r A B e" := (a_fn r A B e) (in custom exp at level 1, r constr at level 0, A custom exp at level 0, B custom exp at level 0, e custom exp at level 60) : mcpts_scope.
   Notation "f x .. y" := (a_app .. (a_app f x) .. y) (in custom exp at level 40, f custom exp, x custom exp at next level, y custom exp at next level) : mcpts_scope.
-  Notation "'#' n" := (a_var n) (in custom exp at level 0, n constr at level 0, format "'#' n") : mcpts_scope.
-
+  Notation "'↑' r A" := (a_upshift r A) (in custom exp at level 1, r constr at level 0, A custom exp at level 60) : mcpts_scope.
+  Notation "'susp' r M" := (a_susp r M) (in custom exp at level 1, r constr at level 0, M custom exp at level 60) : mcpts_scope.
+  Notation "'force' r M" := (a_force r M) (in custom exp at level 1, r constr at level 0, M custom exp at level 60) : mcpts_scope.
+  Notation "'#' n" := (a_var n) (in custom exp at level 0, n constr at level 0, format "'#' n") : mcpts_scope.  
+  
   Notation "'Id'" := a_id (in custom exp at level 0) : mcpts_scope.
   Notation "'Wk'" := a_weaken (in custom exp at level 0) : mcpts_scope.
   Notation "σ ∘ τ" := (a_compose σ τ) (in custom exp at level 40, right associativity, format "σ ∘ τ") : mcpts_scope.
@@ -242,6 +346,10 @@ Module Syntax_Notations.
   Notation "'Π' r A B" := (nf_pi r A B) (in custom nf at level 2, r constr at level 0, A custom nf at level 1, B custom nf at level 60) : mcpts_scope.
   Notation "'λ' r A B e" := (nf_fn r A B e) (in custom nf at level 2, r constr at level 0, A custom nf at level 1, B custom nf at level 1, e custom nf at level 60) : mcpts_scope.
   Notation "f x .. y" := (ne_app .. (ne_app f x) .. y) (in custom nf at level 40, f custom nf, x custom nf at next level, y custom nf at next level) : mcpts_scope.
+  Notation "'↑' r A" := (nf_upshift r A) (in custom exp at level 1, r constr at level 0, A custom exp at level 60) : mcpts_scope.
+  Notation "'susp' r M" := (nf_susp r M) (in custom exp at level 1, r constr at level 0, M custom exp at level 60) : mcpts_scope.
+  Notation "'force' r M" := (ne_force r M) (in custom exp at level 1, r constr at level 0, M custom exp at level 60) : mcpts_scope.
+  Notation "'#' n" := (a_var n) (in custom exp at level 0, n constr at level 0, format "'#' n") : mcpts_scope.
   Notation "'#' n" := (ne_var n) (in custom nf at level 0, n constr at level 0, format "'#' n") : mcpts_scope.
   Notation "'⇑' M" := (nf_neut M) (in custom nf at level 0, M custom nf at level 99, format "'⇑'  M") : mcpts_scope.
 End Syntax_Notations.
