theories/PtsSignature/Adjoint.v
@@ -1,0 +1,19 @@
+From Coq Require Import Relation_Definitions RelationClasses.
+
+From McPTS.PtsSignature Require Import Signatures.
+From McPTS.Core Require Import Base.
+
+Record AdjSig : Type :=
+  mkAdjPts {
+      Modes : Set;
+      Mode_preorder : relation Modes;
+      Preorder_refl : forall m, Mode_preorder m m;
+      Preorder_trans : forall m1 m2 m3, Mode_preorder m1 m2 -> Mode_preorder m2 m3 -> Mode_preorder m1 m3;
+      
+      Mode_to_PtsSig : Modes -> PtsSig;
+      Ru_upshift : forall m1 m2, Mode_preorder m1 m2 -> Mode_to_PtsSig m1 -> Mode_to_PtsSig m2 -> Set;
+    }.
+
+Coercion Mode_to_PtsSig : Modes >-> PtsSig.
+
+Notation "m1 ⪯ m2 ∈ P" := (Mode_preorder P m1 m2) (in custom judg at level 80, m1 constr, m2 constr, P constr) : type_scope.
